

$$\text{eq 22} \Rightarrow a' = \sigma(wa + b)$$

$$\text{eq 23} \Rightarrow a' = \frac{1}{1 + e^{-(\sum_j w_j a_j + b)}}$$

$$a' = \sigma(wa + b)$$

$a \rightarrow$ activation vector

$$a = \begin{bmatrix} a_1 \\ a_2 \\ \vdots \\ a_n \end{bmatrix}$$

$w \Rightarrow$ weight vectorized

$$w = [w_1, w_2, \dots, w_n]$$

$$wa = [w_1, w_2, \dots, w_n] \begin{bmatrix} a_1 \\ a_2 \\ \vdots \\ a_n \end{bmatrix}$$

$$= w_1 a_1 + w_2 a_2 + \dots + w_n a_n$$

$$w.a = \sum_i w_i a_i = \sum_j w_j a_j$$

$$\sigma(wa + b) = \sigma\left(\sum_j w_j a_j + b\right)$$

$$= \frac{1}{1 + e^{-(\sum_j w_j a_j + b)}} = \text{eq 23}$$

Hence proved,,